IMLTT/typed/checked/TypeChecker.lean
@@ -47,7 +47,8 @@ mutual
       return .up <| IsType.univ_elim has_type_A.down
   termination_by structural f => f
 
-  def has_type : (fuel : Nat) -> (Γ : Ctx n) → (t : Tm n) → (T : Tm n) → Except String (PLift (Γ ⊢ t ∶ T))
+  def has_type : (fuel : Nat) → (Γ : Ctx n) →
+      (t : Tm n) → (T : Tm n) → Except String (PLift (Γ ⊢ t ∶ T))
     | 0, _, _, _ => .error "has_type: out of fuel"
     | f+1, Γ, ⋆, 𝟙 => do
       let ctx_ok ← is_ctx (is_type f) Γ
@@ -76,13 +77,14 @@ mutual
       have has_type_T : (Γ ⬝ T) ⊢ v(0) ∶ (T⌊↑ₚidₚ⌋) := HasType.var is_type_T.down
       return .up <| HasType.ty_conv has_type_T eq_type.down
     | f+1, Γ ⬝ T, v(⟨i+1,_⟩), T' => do
+      -- the following infer_type always succeeds in valid contexts
       let ⟨T'', h⟩ ← infer_type f Γ v(.mk i (by simp_all only [Nat.add_lt_add_iff_right]))
-      let is_type_T' ← is_type f _ Γ T''
       let is_type_T ← is_type f _ Γ T
       let weak := HasType.weak h is_type_T.down
       let eq_type ← is_eq_type f (Γ ⬝ T) (T''⌊↑ₚidₚ⌋) T'
       return .up <| HasType.ty_conv weak eq_type.down
     | f+1, Γ ⬝ T, t, v(⟨i,_⟩) =>
+      -- FIXME: this should be possible! Γ ⬝ 𝒰 ⬝ Πv(0);v(1) ⊢ λv(1);v(0) ∶ v(0)
       .error s!"has_type: can't show {t}∶v({i}) if v({i}) is unkown value of type {T}"
     | f+1, Γ, λA;t, ΠA';B' => do
       let eq_type ← is_eq_type f Γ A A'
@@ -135,22 +137,53 @@ mutual
       let eq_type_A ← is_eq_type f (Γ) A A'
       let eq_type_B ← is_eq_type f (Γ ⬝ A) B B'
       return .up <| IsEqualType.sigma_form_eq eq_type_A.down eq_type_B.down
+    | f+1, Γ ⬝ T, v(i), T' => do
+      let ⟨𝒰, _⟩ ← infer_type f (Γ ⬝ T) v(i)
+        | .error s!"is_eq_type: expected a 𝒰 at v({i})"
+      let eq_term_in_𝒰 ← is_eq_term f (Γ ⬝ T) v(⟨i,_⟩) T' 𝒰
+      return .up <| IsEqualType.univ_elim_eq eq_term_in_𝒰.down
+    | f+1, Γ, g◃x, T => do
+      /-let ⟨Π_;_, _⟩ ← infer_type f Γ g
+        | .error s!"is_eq_type: expected a lambda term at {g}"-/
+      let eq_term_in_𝒰 ← is_eq_term f Γ (g◃x) T 𝒰
+      return .up <| IsEqualType.univ_elim_eq eq_term_in_𝒰.down
     | f+1, Γ, a₁ ≃[A] a₃, a₂ ≃[A'] a₄ => do
       let eq_type_A ← is_eq_type f Γ A A'
-      let eq_term <- is_eq_term f Γ A a₁ a₂
-      let eq_term' <- is_eq_term f Γ A' a₃ a₄
+      let eq_term <- is_eq_term f Γ a₁ a₂ A
+      let eq_term' <- is_eq_term f Γ a₃ a₄ A'
       return .up <| IsEqualType.iden_form_eq eq_type_A.down eq_term.down eq_term'.down
-    | _, _, A, B => .error s!"is_eq_type: unsupported pattern for either side {A} ≡ {B}"
+    | f+1, Γ, T, T' => do
+      let is_eq_symm ← is_eq_type f Γ T' T
+      return .up <| IsEqualType.type_symm is_eq_symm.down
+    --| _, _, A, B => .error s!"is_eq_type: unsupported pattern for either side {A} ≡ {B}"
   termination_by structural f => f
 
   def is_eq_term : (fuel: Nat) -> (Γ : Ctx n) ->
-      (A : Tm n) → (a : Tm n) → (a' : Tm n) → Except String (PLift (Γ ⊢ a ≡ a' ∶ A))
+      (a : Tm n) → (a' : Tm n) → (A : Tm n) → Except String (PLift (Γ ⊢ a ≡ a' ∶ A))
     | 0, _, _, _, _ => .error "is_eq_term: out of fuel"
-    | f+1, Γ, 𝟙, ⋆, ⋆ => do
+    | f+1, Γ, ⋆, ⋆, 𝟙 => do
       let ctx_ok ← is_ctx (is_type f) Γ
       return .up <| IsEqualTerm.unit_intro_eq ctx_ok.down
-    | _, _, A, a, a' =>
-      .error s!"is_eq_type: unsupported pattern for either side or type {a} ≃[{A}] {a'}"
+    | f+1, Γ, 𝒩, 𝒩, 𝒰 => do
+      let ctx_ok ← is_ctx (is_type f) Γ
+      return .up <| IsEqualTerm.univ_nat_eq ctx_ok.down
+    | f+1, Γ ⬝ T, v(0), v(0), T' => do
+      let is_type_T ← is_type f _ Γ T
+      let is_eq_T_T' ← is_eq_type f (Γ ⬝ T) (T⌊↑ₚidₚ⌋) T'
+      have := IsEqualTerm.var_eq is_type_T.down
+      return .up <| IsEqualTerm.ty_conv_eq this is_eq_T_T'.down
+    | f+1, Γ, (λA;b)◃x, t, T => do
+      let ⟨Π_;B, _⟩ ← infer_type f Γ (λA;b)
+        | .error s!"is_eq_term: could not infer type of {λA;b}"
+      let has_type_x ← has_type f Γ x A
+      let has_type_b ← has_type f (Γ ⬝ A) b B
+      have pi_comp := IsEqualTerm.pi_comp has_type_b.down has_type_x.down
+      let is_eq_term_b ← is_eq_term f Γ (b⌈x⌉₀) t (B⌈x⌉₀)
+      let is_eq_type_B_T ← is_eq_type f Γ (B⌈x⌉₀) T
+      have := IsEqualTerm.term_trans pi_comp is_eq_term_b.down
+      return .up <| IsEqualTerm.ty_conv_eq this is_eq_type_B_T.down
+    | _, _, a, a', A =>
+      .error s!"is_eq_term: unsupported pattern for either side or type {a} ≃[{A}] {a'}"
   termination_by structural f => f
 
   def infer_type : (fuel : Nat) → (Γ : Ctx n) → (t : Tm n) → Except String (Σ' T, Γ ⊢ t ∶ T)
@@ -233,13 +266,28 @@ def ret_id : Tm n := (λ𝒰;(λv(0);v(0)))
 #eval has_type fuel (ε ⬝ 𝒩 ⬝ 𝟙) ((λ𝒩;𝓈(v(0))&((λ𝒰;(λv(0);v(0))◃𝒩)◃v(0)))◃v(1)) (Σ𝒩;𝒩)
 #eval has_type fuel (ε ⬝ 𝒩 ⬝ 𝟙) ((λ𝒩;𝓈(v(0))&((λ𝒰;(λv(0);v(0))◃𝒩)◃v(0)))◃v(1)) (Σ𝒩;𝒩)
 
-#eval has_type fuel (ε ⬝ 𝒩 ⬝ 𝟙) (((λ𝒰;(λv(0);v(0)))◃𝒩)◃v(1)) 𝒩
+#reduce has_type fuel (ε ⬝ 𝒩 ⬝ 𝟙) (((λ𝒰;(λv(0);v(0)))◃𝒩)◃v(1)) 𝒩
 
 #eval has_type fuel (ε ⬝ 𝒩) ((λ𝒩;v(0))◃v(0)) 𝒩
 #eval has_type fuel (ε ⬝ 𝒩) (((λ𝒰;v(0)))◃𝒩) 𝒰
 #eval has_type fuel (ε ⬝ 𝒩) ((λ(((λ𝒰;v(0)))◃𝒩);v(0))◃v(0)) 𝒩
 
+#eval is_eq_type fuel (ε ⬝ 𝒰) v(0) v(0)
+
+#eval has_type fuel (ε ⬝ 𝒰) (((λ𝒰;(λv(0);v(0)))◃𝒩)◃𝓏) 𝒩
+#eval has_type fuel (ε ⬝ 𝒰 ⬝ Πv(0);v(1)) (((v(0) ◃ (λv(0);v(0)))◃𝒩)◃𝓏) 𝒩
+
+/-
+Γ ⬝ A ⬝ B ⬝ C ⊢ (λ(ΠB;C);(λ(ΠA;B);(λA; v(2)◃(v(1)◃v(0)))) : ΠA;C
+Γ ⬝ (A : 𝒰) ⬝ (B : 𝒰) ⬝ (C : 𝒰) ⊢ (λ(g : ΠB;C);(λ(f : ΠA;B);(λ(x : A); g◃(f◃x))) : ΠA;C
+-/
+#eval has_type fuel (ε ⬝ 𝒰 ⬝ 𝒰 ⬝ 𝒰)
+    (λ(Πv(1);v(0+1));(λ(Πv(2+1);v(1+1+1));(λv(2+1+1); v(2)◃(v(1)◃v(0))))) (Πv(2);v(1))
+
 #reduce is_eq_type fuel (ε ⬝ 𝒩) (((λ𝒰;v(0)))◃𝒩) 𝒩
 
 example : ε ⊢ (Tm.lam 𝒩 𝓈(v(0))) ∶ Tm.pi 𝒩 𝒩 :=
   ((has_type fuel ε (Tm.lam 𝒩 𝓈(v(0))) (Tm.pi 𝒩 𝒩)).toOption.get (by native_decide)).down
+
+
+#check Lean.Expr
